common/Smallstep.v
@@ -474,13 +474,14 @@ End CLOSURES.
 
 (** The general form of a transition semantics. *)
 
-Record semantics : Type := mksemantics {
+Record semantics : Type := mk_semantics {
   state: Type;
   funtype: Type;
   vartype: Type;
   step :> Genv.t funtype vartype -> state -> trace -> state -> Prop;
   initial_state: state -> Prop;
-  final_state: state -> int -> Prop
+  final_state: state -> int -> Prop;
+  genv: Genv.t funtype vartype
 }.
 
 Definition globalenv (L: semantics) : Type := Genv.t (funtype L) (vartype L).
@@ -489,7 +490,7 @@ Definition globalenv (L: semantics) : Type := Genv.t (funtype L) (vartype L).
 
 (** The general form of a forward simulation. *)
 
-Record forward_simulation (L1 L2: semantics) (ge1: globalenv L1) (ge2: globalenv L2) :=
+Record forward_simulation (L1 L2: semantics) :=
   mk_forward_simulation {
     fsim_index: Type;
     fsim_order: fsim_index -> fsim_index -> Prop;
@@ -502,13 +503,13 @@ Record forward_simulation (L1 L2: semantics) (ge1: globalenv L1) (ge2: globalenv
       forall i s1 s2 r, 
       fsim_match_states i s1 s2 -> final_state L1 s1 r -> final_state L2 s2 r;
     fsim_simulation:
-      forall s1 t s1', L1 ge1 s1 t s1' ->
+      forall s1 t s1', L1 (genv L1) s1 t s1' ->
       forall i s2, fsim_match_states i s1 s2 ->
       exists i', exists s2',
-         (plus L2 ge2 s2 t s2' \/ (star L2 ge2 s2 t s2' /\ fsim_order i' i))
+         (plus L2 (genv L2) s2 t s2' \/ (star L2 (genv L2) s2 t s2' /\ fsim_order i' i))
       /\ fsim_match_states i' s1' s2';
     fsim_symbols_preserved:
-      forall id, Genv.find_symbol ge1 id = Genv.find_symbol ge2 id
+      forall id, Genv.find_symbol (genv L1) id = Genv.find_symbol (genv L2) id
   }.
 
 Implicit Arguments forward_simulation [].
@@ -516,10 +517,10 @@ Implicit Arguments forward_simulation [].
 (** An alternate form of the simulation diagram *)
 
 Lemma fsim_simulation':
-  forall L1 L2 ge1 ge2 (S: forward_simulation L1 L2 ge1 ge2),
-  forall i s1 t s1', L1 ge1 s1 t s1' ->
+  forall L1 L2 (S: forward_simulation L1 L2),
+  forall i s1 t s1', L1 (genv L1) s1 t s1' ->
   forall s2, S i s1 s2 ->
-  (exists i', exists s2', plus L2 ge2 s2 t s2' /\ S i' s1' s2')
+  (exists i', exists s2', plus L2 (genv L2) s2 t s2' /\ S i' s1' s2')
   \/ (exists i', fsim_order S i' i /\ t = E0 /\ S i' s1' s2).
 Proof.
   intros. exploit fsim_simulation; eauto. 
@@ -538,11 +539,9 @@ Section FORWARD_SIMU_DIAGRAMS.
 
 Variable L1: semantics.
 Variable L2: semantics.
-Variable ge1: globalenv L1.
-Variable ge2: globalenv L2.
 
 Hypothesis symbols_preserved:
-  forall id, Genv.find_symbol ge1 id = Genv.find_symbol ge2 id.
+  forall id, Genv.find_symbol (genv L1) id = Genv.find_symbol (genv L2) id.
 
 Variable match_states: state L1 -> state L2 -> Prop.
 
@@ -572,13 +571,13 @@ Variable order: state L1 -> state L1 -> Prop.
 Hypothesis order_wf: well_founded order.
 
 Hypothesis simulation:
-  forall s1 t s1', L1 ge1 s1 t s1' ->
+  forall s1 t s1', L1 (genv L1) s1 t s1' ->
   forall s2, match_states s1 s2 ->
   exists s2',
-  (plus L2 ge2 s2 t s2' \/ (star L2 ge2 s2 t s2' /\ order s1' s1))
+  (plus L2 (genv L2) s2 t s2' \/ (star L2 (genv L2) s2 t s2' /\ order s1' s1))
   /\ match_states s1' s2'.
 
-Lemma simulation_star_wf: forward_simulation L1 L2 ge1 ge2.
+Lemma simulation_star_wf: forward_simulation L1 L2.
 Proof.
   apply mk_forward_simulation with
     (fsim_order := order)
@@ -602,12 +601,12 @@ Section SIMULATION_STAR.
 Variable measure: state L1 -> nat.
 
 Hypothesis simulation:
-  forall s1 t s1', L1 ge1 s1 t s1' ->
+  forall s1 t s1', L1 (genv L1) s1 t s1' ->
   forall s2, match_states s1 s2 ->
-  (exists s2', plus L2 ge2 s2 t s2' /\ match_states s1' s2')
+  (exists s2', plus L2 (genv L2) s2 t s2' /\ match_states s1' s2')
   \/ (measure s1' < measure s1 /\ t = E0 /\ match_states s1' s2)%nat.
 
-Lemma simulation_star_preservation: forward_simulation L1 L2 ge1 ge2.
+Lemma simulation_star_preservation: forward_simulation L1 L2.
 Proof.
   apply simulation_star_wf with (ltof _ measure).
   apply well_founded_ltof.
@@ -624,11 +623,11 @@ End SIMULATION_STAR.
 Section SIMULATION_PLUS.
 
 Hypothesis simulation:
-  forall s1 t s1', L1 ge1 s1 t s1' ->
+  forall s1 t s1', L1 (genv L1) s1 t s1' ->
   forall s2, match_states s1 s2 ->
-  exists s2', plus L2 ge2 s2 t s2' /\ match_states s1' s2'.
+  exists s2', plus L2 (genv L2) s2 t s2' /\ match_states s1' s2'.
 
-Lemma simulation_plus_preservation: forward_simulation L1 L2 ge1 ge2.
+Lemma simulation_plus_preservation: forward_simulation L1 L2.
 Proof.
   apply simulation_star_preservation with (measure := fun _ => O).
   intros. exploit simulation; eauto.
@@ -642,11 +641,11 @@ End SIMULATION_PLUS.
 Section SIMULATION_STEP.
 
 Hypothesis simulation:
-  forall s1 t s1', L1 ge1 s1 t s1' ->
+  forall s1 t s1', L1 (genv L1) s1 t s1' ->
   forall s2, match_states s1 s2 ->
-  exists s2', L2 ge2 s2 t s2' /\ match_states s1' s2'.
+  exists s2', L2 (genv L2) s2 t s2' /\ match_states s1' s2'.
 
-Lemma simulation_step: forward_simulation L1 L2 ge1 ge2.
+Lemma simulation_step: forward_simulation L1 L2.
 Proof.
   apply simulation_plus_preservation. 
   intros. exploit simulation; eauto. intros [s2' [A B]].
@@ -666,12 +665,12 @@ Section SIMULATION_OPT.
 Variable measure: state L1 -> nat.
 
 Hypothesis simulation:
-  forall s1 t s1', L1 ge1 s1 t s1' ->
+  forall s1 t s1', L1 (genv L1) s1 t s1' ->
   forall s2, match_states s1 s2 ->
-  (exists s2', L2 ge2 s2 t s2' /\ match_states s1' s2')
+  (exists s2', L2 (genv L2) s2 t s2' /\ match_states s1' s2')
   \/ (measure s1' < measure s1 /\ t = E0 /\ match_states s1' s2)%nat.
 
-Lemma simulation_opt_preservation: forward_simulation L1 L2 ge1 ge2.
+Lemma simulation_opt_preservation: forward_simulation L1 L2.
 Proof.
   apply simulation_star_preservation with measure.
   intros. exploit simulation; eauto. intros [[s2' [A B]] | [A [B C]]].
@@ -689,14 +688,12 @@ Section SIMULATION_SEQUENCES.
 
 Variable L1: semantics.
 Variable L2: semantics.
-Variable ge1: globalenv L1.
-Variable ge2: globalenv L2.
-Variable S: forward_simulation L1 L2 ge1 ge2.
+Variable S: forward_simulation L1 L2.
 
 Lemma simulation_star:
-  forall s1 t s1', star L1 ge1 s1 t s1' ->
+  forall s1 t s1', star L1 (genv L1) s1 t s1' ->
   forall i s2, S i s1 s2 ->
-  exists i', exists s2', star L2 ge2 s2 t s2' /\ S i' s1' s2'.
+  exists i', exists s2', star L2 (genv L2) s2 t s2' /\ S i' s1' s2'.
 Proof.
   induction 1; intros.
   exists i; exists s2; split; auto. apply star_refl.
@@ -707,9 +704,9 @@ Proof.
 Qed.
 
 Lemma simulation_plus:
-  forall s1 t s1', plus L1 ge1 s1 t s1' ->
+  forall s1 t s1', plus L1 (genv L1) s1 t s1' ->
   forall i s2, S i s1 s2 ->
-  (exists i', exists s2', plus L2 ge2 s2 t s2' /\ S i' s1' s2')
+  (exists i', exists s2', plus L2 (genv L2) s2 t s2' /\ S i' s1' s2')
   \/ (exists i', clos_trans _ (fsim_order S) i' i /\ t = E0 /\ S i' s1' s2).
 Proof.
   induction 1 using plus_ind2; intros.
@@ -730,12 +727,12 @@ Qed.
 
 Lemma simulation_forever_silent:
   forall i s1 s2,
-  forever_silent L1 ge1 s1 -> S i s1 s2 ->
-  forever_silent L2 ge2 s2.
+  forever_silent L1 (genv L1) s1 -> S i s1 s2 ->
+  forever_silent L2 (genv L2) s2.
 Proof.
   assert (forall i s1 s2,
-          forever_silent L1 ge1 s1 -> S i s1 s2 ->
-          forever_silent_N L2 (fsim_order S) ge2 i s2).
+          forever_silent L1 (genv L1) s1 -> S i s1 s2 ->
+          forever_silent_N L2 (fsim_order S) (genv L2) i s2).
     cofix COINDHYP; intros.
     inv H. destruct (fsim_simulation S _ _ _ H1 _ _ H0) as [i' [s2' [A B]]].
     destruct A as [C | [C D]].
@@ -746,8 +743,8 @@ Qed.
 
 Lemma simulation_forever_reactive:
   forall i s1 s2 T,
-  forever_reactive L1 ge1 s1 T -> S i s1 s2 ->
-  forever_reactive L2 ge2 s2 T.
+  forever_reactive L1 (genv L1) s1 T -> S i s1 s2 ->
+  forever_reactive L2 (genv L2) s2 T.
 Proof.
   cofix COINDHYP; intros.
   inv H. 
@@ -764,11 +761,8 @@ Section COMPOSE_SIMULATIONS.
 Variable L1: semantics.
 Variable L2: semantics.
 Variable L3: semantics.
-Variable ge1: globalenv L1.
-Variable ge2: globalenv L2.
-Variable ge3: globalenv L3.
-Variable S12: forward_simulation L1 L2 ge1 ge2.
-Variable S23: forward_simulation L2 L3 ge2 ge3.
+Variable S12: forward_simulation L1 L2.
+Variable S23: forward_simulation L2 L3.
 
 Let ff_index : Type := (fsim_index S23 * fsim_index S12)%type.
 
@@ -778,7 +772,7 @@ Let ff_order : ff_index -> ff_index -> Prop :=
 Let ff_match_states (i: ff_index) (s1: state L1) (s3: state L3) : Prop :=
   exists s2, S12 (snd i) s1 s2 /\ S23 (fst i) s2 s3.
 
-Lemma compose_forward_simulation: forward_simulation L1 L3 ge1 ge3.
+Lemma compose_forward_simulation: forward_simulation L1 L3.
 Proof.
   apply mk_forward_simulation with (fsim_order := ff_order) (fsim_match_states := ff_match_states).
 (* well founded *)
@@ -807,7 +801,7 @@ Proof.
   right; split. subst t; apply star_refl. red. right. auto. 
   exists s3; auto.
 (* symbols *)
-  intros. transitivity (Genv.find_symbol ge2 id); apply fsim_symbols_preserved; auto.
+  intros. transitivity (Genv.find_symbol (genv L2) id); apply fsim_symbols_preserved; auto.
 Qed.
 
 End COMPOSE_SIMULATIONS.
@@ -831,7 +825,7 @@ Qed.
 
 (** The general form of a backward simulation. *)
 
-Record backward_simulation (L1 L2: semantics) (ge1: globalenv L1) (ge2: globalenv L2) :=
+Record backward_simulation (L1 L2: semantics) :=
   mk_backward_simulation {
     bsim_index: Type;
     bsim_order: bsim_index -> bsim_index -> Prop;
@@ -844,23 +838,23 @@ Record backward_simulation (L1 L2: semantics) (ge1: globalenv L1) (ge2: globalen
       exists i, exists s1', initial_state L1 s1' /\ bsim_match_states i s1' s2;
     bsim_match_final_states:
       forall i s1 s2 r, 
-      bsim_match_states i s1 s2 -> safe L1 ge1 s1 -> final_state L2 s2 r -> 
-      exists s1', star L1 ge1 s1 E0 s1' /\ final_state L1 s1' r;
+      bsim_match_states i s1 s2 -> safe L1 (genv L1) s1 -> final_state L2 s2 r -> 
+      exists s1', star L1 (genv L1) s1 E0 s1' /\ final_state L1 s1' r;
     bsim_progress:
       forall i s1 s2, 
-      bsim_match_states i s1 s2 -> safe L1 ge1 s1 ->
+      bsim_match_states i s1 s2 -> safe L1 (genv L1) s1 ->
       (exists r, final_state L2 s2 r) \/
-      (exists t, exists s2', L2 ge2 s2 t s2');
+      (exists t, exists s2', L2 (genv L2) s2 t s2');
     bsim_simulation:
-      forall s2 t s2', L2 ge2 s2 t s2' ->
-      forall i s1, bsim_match_states i s1 s2 -> safe L1 ge1 s1 ->
+      forall s2 t s2', L2 (genv L2) s2 t s2' ->
+      forall i s1, bsim_match_states i s1 s2 -> safe L1 (genv L1) s1 ->
       exists i', exists s1',
-         (plus L1 ge1 s1 t s1' \/ (star L1 ge1 s1 t s1' /\ bsim_order i' i))
+         (plus L1 (genv L1) s1 t s1' \/ (star L1 (genv L1) s1 t s1' /\ bsim_order i' i))
       /\ bsim_match_states i' s1' s2';
     bsim_traces:
-      forall s2 t s2', L2 ge2 s2 t s2' -> (length t <= 1)%nat;
+      forall s2 t s2', L2 (genv L2) s2 t s2' -> (length t <= 1)%nat;
     bsim_symbols_preserved:
-      forall id, Genv.find_symbol ge1 id = Genv.find_symbol ge2 id
+      forall id, Genv.find_symbol (genv L1) id = Genv.find_symbol (genv L2) id
   }.
 
 Implicit Arguments backward_simulation [].
@@ -868,10 +862,10 @@ Implicit Arguments backward_simulation [].
 (** An alternate form of the simulation diagram *)
 
 Lemma bsim_simulation':
-  forall L1 L2 ge1 ge2 (S: backward_simulation L1 L2 ge1 ge2),
-  forall i s2 t s2', L2 ge2 s2 t s2' ->
-  forall s1, S i s1 s2 -> safe L1 ge1 s1 ->
-  (exists i', exists s1', plus L1 ge1 s1 t s1' /\ S i' s1' s2')
+  forall L1 L2 (S: backward_simulation L1 L2),
+  forall i s2 t s2', L2 (genv L2) s2 t s2' ->
+  forall s1, S i s1 s2 -> safe L1 (genv L1) s1 ->
+  (exists i', exists s1', plus L1 (genv L1) s1 t s1' /\ S i' s1' s2')
   \/ (exists i', bsim_order S i' i /\ t = E0 /\ S i' s1 s2').
 Proof.
   intros. exploit bsim_simulation; eauto. 
@@ -890,14 +884,12 @@ Section BACKWARD_SIMU_DIAGRAMS.
 
 Variable L1: semantics.
 Variable L2: semantics.
-Variable ge1: globalenv L1.
-Variable ge2: globalenv L2.
 
 Hypothesis symbols_preserved:
-  forall id, Genv.find_symbol ge1 id = Genv.find_symbol ge2 id.
+  forall id, Genv.find_symbol (genv L1) id = Genv.find_symbol (genv L2) id.
 
 Hypothesis length_traces:
-  forall s2 t s2', L2 ge2 s2 t s2' -> (length t <= 1)%nat.
+  forall s2 t s2', L2 (genv L2) s2 t s2' -> (length t <= 1)%nat.
 
 Variable match_states: state L1 -> state L2 -> Prop.
 
@@ -914,18 +906,18 @@ Hypothesis match_final_states:
 
 Hypothesis progress:
   forall s1 s2, 
-  match_states s1 s2 -> safe L1 ge1 s1 ->
+  match_states s1 s2 -> safe L1 (genv L1) s1 ->
   (exists r, final_state L2 s2 r) \/
-  (exists t, exists s2', L2 ge2 s2 t s2').
+  (exists t, exists s2', L2 (genv L2) s2 t s2').
 
 Section BACKWARD_SIMULATION_PLUS.
 
 Hypothesis simulation:
-  forall s2 t s2', L2 ge2 s2 t s2' ->
-  forall s1, match_states s1 s2 -> safe L1 ge1 s1 ->
-  exists s1', plus L1 ge1 s1 t s1' /\ match_states s1' s2'.
+  forall s2 t s2', L2 (genv L2) s2 t s2' ->
+  forall s1, match_states s1 s2 -> safe L1 (genv L1) s1 ->
+  exists s1', plus L1 (genv L1) s1 t s1' /\ match_states s1' s2'.
 
-Lemma backward_simulation_plus: backward_simulation L1 L2 ge1 ge2.
+Lemma backward_simulation_plus: backward_simulation L1 L2.
 Proof.
   apply mk_backward_simulation with
     (bsim_order := fun (x y: unit) => False)
@@ -948,28 +940,26 @@ Section BACKWARD_SIMULATION_SEQUENCES.
 
 Variable L1: semantics.
 Variable L2: semantics.
-Variable ge1: globalenv L1.
-Variable ge2: globalenv L2.
-Variable S: backward_simulation L1 L2 ge1 ge2.
+Variable S: backward_simulation L1 L2.
 
 Lemma bsim_E0_star:
-  forall s2 s2', star L2 ge2 s2 E0 s2' ->
-  forall i s1, S i s1 s2 -> safe L1 ge1 s1 ->
-  exists i', exists s1', star L1 ge1 s1 E0 s1' /\ S i' s1' s2'.
+  forall s2 s2', star L2 (genv L2) s2 E0 s2' ->
+  forall i s1, S i s1 s2 -> safe L1 (genv L1) s1 ->
+  exists i', exists s1', star L1 (genv L1) s1 E0 s1' /\ S i' s1' s2'.
 Proof.
   intros s20 s20' STAR0. pattern s20, s20'. eapply star_E0_ind; eauto.
 (* base case *)
   intros. exists i; exists s1; split; auto. apply star_refl.
 (* inductive case *)
   intros. exploit bsim_simulation; eauto. intros [i' [s1' [A B]]].
-  assert (star L1 ge1 s0 E0 s1'). intuition. apply plus_star; auto. 
+  assert (star L1 (genv L1) s0 E0 s1'). intuition. apply plus_star; auto. 
   exploit H0. eauto. eapply star_safe; eauto. intros [i'' [s1'' [C D]]].
   exists i''; exists s1''; split; auto. eapply star_trans; eauto.
 Qed.
 
 Lemma bsim_safe:
   forall i s1 s2,
-  S i s1 s2 -> safe L1 ge1 s1 -> safe L2 ge2 s2.
+  S i s1 s2 -> safe L1 (genv L1) s1 -> safe L2 (genv L2) s2.
 Proof.
   intros; red; intros. 
   exploit bsim_E0_star; eauto. intros [i' [s1' [A B]]].
@@ -977,9 +967,9 @@ Proof.
 Qed.
 
 Lemma bsim_E0_plus:
-  forall s2 t s2', plus L2 ge2 s2 t s2' -> t = E0 ->
-  forall i s1, S i s1 s2 -> safe L1 ge1 s1 ->
-     (exists i', exists s1', plus L1 ge1 s1 E0 s1' /\ S i' s1' s2')
+  forall s2 t s2', plus L2 (genv L2) s2 t s2' -> t = E0 ->
+  forall i s1, S i s1 s2 -> safe L1 (genv L1) s1 ->
+     (exists i', exists s1', plus L1 (genv L1) s1 E0 s1' /\ S i' s1' s2')
   \/ (exists i', clos_trans _ (bsim_order S) i' i /\ S i' s1 s2').
 Proof.
   induction 1 using plus_ind2; intros; subst t.
@@ -999,8 +989,8 @@ Proof.
 Qed.
 
 Lemma star_non_E0_split:
-  forall s2 t s2', star L2 ge2 s2 t s2' -> (length t = 1)%nat ->
-  exists s2x, exists s2y, star L2 ge2 s2 E0 s2x /\ L2 ge2 s2x t s2y /\ star L2 ge2 s2y E0 s2'.
+  forall s2 t s2', star L2 (genv L2) s2 t s2' -> (length t = 1)%nat ->
+  exists s2x, exists s2y, star L2 (genv L2) s2 E0 s2x /\ L2 (genv L2) s2x t s2y /\ star L2 (genv L2) s2y E0 s2'.
 Proof.
   induction 1; intros.
   simpl in H; discriminate.
@@ -1023,11 +1013,8 @@ Section COMPOSE_BACKWARD_SIMULATIONS.
 Variable L1: semantics.
 Variable L2: semantics.
 Variable L3: semantics.
-Variable ge1: globalenv L1.
-Variable ge2: globalenv L2.
-Variable ge3: globalenv L3.
-Variable S12: backward_simulation L1 L2 ge1 ge2.
-Variable S23: backward_simulation L2 L3 ge2 ge3.
+Variable S12: backward_simulation L1 L2.
+Variable S23: backward_simulation L2 L3.
 
 Let bb_index : Type := (bsim_index S12 * bsim_index S23)%type.
 
@@ -1036,7 +1023,7 @@ Let bb_order : bb_index -> bb_index -> Prop :=
 
 Inductive bb_match_states: bb_index -> state L1 -> state L3 -> Prop :=
   | bb_match_later: forall i1 i2 s1 s3 s2x s2y,
-      S12 i1 s1 s2x -> star L2 ge2 s2x E0 s2y -> S23 i2 s2y s3 ->
+      S12 i1 s1 s2x -> star L2 (genv L2) s2x E0 s2y -> S23 i2 s2y s3 ->
       bb_match_states (i1, i2) s1 s3.
 
 Lemma bb_match_at: forall i1 i2 s1 s3 s2,
@@ -1047,10 +1034,10 @@ Proof.
 Qed. 
 
 Lemma bb_simulation_base:
-  forall s3 t s3', L3 ge3 s3 t s3' ->
-  forall i1 s1 i2 s2, S12 i1 s1 s2 -> S23 i2 s2 s3 -> safe L1 ge1 s1 ->
+  forall s3 t s3', L3 (genv L3) s3 t s3' ->
+  forall i1 s1 i2 s2, S12 i1 s1 s2 -> S23 i2 s2 s3 -> safe L1 (genv L1) s1 ->
   exists i', exists s1',
-    (plus L1 ge1 s1 t s1' \/ (star L1 ge1 s1 t s1' /\ bb_order i' (i1, i2)))
+    (plus L1 (genv L1) s1 t s1' \/ (star L1 (genv L1) s1 t s1' /\ bb_order i' (i1, i2)))
     /\ bb_match_states i' s1' s3'.
 Proof.
   intros.
@@ -1085,10 +1072,10 @@ Proof.
 Qed.
 
 Lemma bb_simulation:
-  forall s3 t s3', L3 ge3 s3 t s3' ->
-  forall i s1, bb_match_states i s1 s3 -> safe L1 ge1 s1 ->
+  forall s3 t s3', L3 (genv L3) s3 t s3' ->
+  forall i s1, bb_match_states i s1 s3 -> safe L1 (genv L1) s1 ->
   exists i', exists s1',
-    (plus L1 ge1 s1 t s1' \/ (star L1 ge1 s1 t s1' /\ bb_order i' i))
+    (plus L1 (genv L1) s1 t s1' \/ (star L1 (genv L1) s1 t s1' /\ bb_order i' i))
     /\ bb_match_states i' s1' s3'.
 Proof.
   intros. inv H0. 
@@ -1114,7 +1101,7 @@ Proof.
   inv H6. left. eapply t_trans; eauto. left; auto.
 Qed.
 
-Lemma compose_backward_simulation: backward_simulation L1 L3 ge1 ge3.
+Lemma compose_backward_simulation: backward_simulation L1 L3.
 Proof.
   apply mk_backward_simulation with (bsim_order := bb_order) (bsim_match_states := bb_match_states).
 (* well founded *)
@@ -1146,7 +1133,7 @@ Proof.
 (* trace length *)
   exact (bsim_traces S23). 
 (* symbols *)
-  intros. transitivity (Genv.find_symbol ge2 id); apply bsim_symbols_preserved; auto.
+  intros. transitivity (Genv.find_symbol (genv L2) id); apply bsim_symbols_preserved; auto.
 Qed.
 
 End COMPOSE_BACKWARD_SIMULATIONS.
@@ -1155,20 +1142,20 @@ End COMPOSE_BACKWARD_SIMULATIONS.
 
 Record sem_receptive (L: semantics) : Prop :=
   mk_sem_receptive {
-    sr_receptive: forall ge s t1 s1 t2,
-      L ge s t1 s1 -> match_traces ge t1 t2 -> exists s2, L ge s t2 s2;
-    sr_traces: forall ge s t s',
-      L ge s t s' -> (length t <= 1)%nat
+    sr_receptive: forall s t1 s1 t2,
+      L (genv L) s t1 s1 -> match_traces (genv L) t1 t2 -> exists s2, L (genv L) s t2 s2;
+    sr_traces: forall s t s',
+      L (genv L) s t s' -> (length t <= 1)%nat
   }.
 
 Record sem_determinate (L: semantics) : Prop :=
   mk_sem_determinate {
-    sd_match: forall ge s t1 s1 t2 s2,
-      L ge s t1 s1 -> L ge s t2 s2 -> match_traces ge t1 t2;
-    sd_determ: forall ge s t s1 s2,
-      L ge s t s1 -> L ge s t s2 -> s1 = s2;
-    sd_traces: forall ge s t s',
-      L ge s t s' -> (length t <= 1)%nat;
+    sd_match: forall s t1 s1 t2 s2,
+      L (genv L) s t1 s1 -> L (genv L) s t2 s2 -> match_traces (genv L) t1 t2;
+    sd_determ: forall s t s1 s2,
+      L (genv L) s t s1 -> L (genv L) s t s2 -> s1 = s2;
+    sd_traces: forall s t s',
+      L (genv L) s t s' -> (length t <= 1)%nat;
     sd_initial_determ: forall s1 s2,
       initial_state L s1 -> initial_state L s2 -> s1 = s2;
     sd_final_nostep: forall ge s r,
@@ -1181,9 +1168,7 @@ Section FORWARD_TO_BACKWARD.
 
 Variable L1: semantics.
 Variable L2: semantics.
-Variable ge1: globalenv L1.
-Variable ge2: globalenv L2.
-Variable FS: forward_simulation L1 L2 ge1 ge2.
+Variable FS: forward_simulation L1 L2.
 
 Hypothesis receptive: sem_receptive L1.
 Hypothesis determinate: sem_determinate L2.
@@ -1192,20 +1177,20 @@ Hypothesis determinate: sem_determinate L2.
 
 Inductive f2b_transitions: state L1 -> state L2 -> Prop :=
   | f2b_trans_final: forall s1 s2 s1' r,
-      star L1 ge1 s1 E0 s1' ->
+      star L1 (genv L1) s1 E0 s1' ->
       final_state L1 s1' r ->
       final_state L2 s2 r ->
       f2b_transitions s1 s2
   | f2b_trans_step: forall s1 s2 s1' t s1'' s2' i' i'',
-      star L1 ge1 s1 E0 s1' ->
-      L1 ge1 s1' t s1'' ->
-      plus L2 ge2 s2 t s2' ->
+      star L1 (genv L1) s1 E0 s1' ->
+      L1 (genv L1) s1' t s1'' ->
+      plus L2 (genv L2) s2 t s2' ->
       FS i' s1' s2 -> 
       FS i'' s1'' s2' ->
       f2b_transitions s1 s2.
 
 Lemma f2b_progress:
-  forall i s1 s2, FS i s1 s2 -> safe L1 ge1 s1 -> f2b_transitions s1 s2.
+  forall i s1 s2, FS i s1 s2 -> safe L1 (genv L1) s1 -> f2b_transitions s1 s2.
 Proof.
   intros i0; pattern i0. apply well_founded_ind with (R := fsim_order FS). 
   apply fsim_order_wf.
@@ -1217,7 +1202,7 @@ Proof.
   eapply fsim_match_final_states; eauto. 
   (* L1 can make one step *)
   exploit (fsim_simulation FS); eauto. intros [i' [s2' [A MATCH']]].
-  assert (B: plus L2 ge2 s2 t s2' \/ (s2' = s2 /\ t = E0 /\ fsim_order FS i' i)).
+  assert (B: plus L2 (genv L2) s2 t s2' \/ (s2' = s2 /\ t = E0 /\ fsim_order FS i' i)).
     intuition.
     destruct (star_inv H0); intuition.
   clear A. destruct B as [PLUS2 | [EQ1 [EQ2 ORDER]]].
@@ -1229,9 +1214,9 @@ Proof.
 Qed.
 
 Lemma fsim_simulation_not_E0:
-  forall s1 t s1', L1 ge1 s1 t s1' -> t <> E0 ->
+  forall s1 t s1', L1 (genv L1) s1 t s1' -> t <> E0 ->
   forall i s2, FS i s1 s2 ->
-  exists i', exists s2', plus L2 ge2 s2 t s2' /\ FS i' s1' s2'.
+  exists i', exists s2', plus L2 (genv L2) s2 t s2' /\ FS i' s1' s2'.
 Proof.
   intros. exploit (fsim_simulation FS); eauto. intros [i' [s2' [A B]]].
   exists i'; exists s2'; split; auto.
@@ -1280,19 +1265,19 @@ Inductive f2b_match_states: f2b_index -> state L1 -> state L2 -> Prop :=
       FS i s1 s2 ->
       f2b_match_states (F2BI_after O) s1 s2
   | f2b_match_before: forall s1 t s1' s2b s2 n s2a i,
-      L1 ge1 s1 t s1' ->  t <> E0 ->
-      star L2 ge2 s2b E0 s2 ->
-      starN L2 ge2 n s2 t s2a ->
+      L1 (genv L1) s1 t s1' ->  t <> E0 ->
+      star L2 (genv L2) s2b E0 s2 ->
+      starN L2 (genv L2) n s2 t s2a ->
       FS i s1 s2b ->
       f2b_match_states (F2BI_before n) s1 s2
   | f2b_match_after: forall n s2 s2a s1 i,
-      starN L2 ge2 (S n) s2 E0 s2a ->
+      starN L2 (genv L2) (S n) s2 E0 s2a ->
       FS i s1 s2a ->
       f2b_match_states (F2BI_after (S n)) s1 s2.
 
 Remark f2b_match_after':
   forall n s2 s2a s1 i,
-  starN L2 ge2 n s2 E0 s2a ->
+  starN L2 (genv L2) n s2 E0 s2a ->
   FS i s1 s2a ->
   f2b_match_states (F2BI_after n) s1 s2.
 Proof.
@@ -1318,12 +1303,12 @@ Qed.
 
 Lemma f2b_determinacy_inv:
   forall s2 t' s2' t'' s2'',
-  L2 ge2 s2 t' s2' -> L2 ge2 s2 t'' s2'' ->
+  L2 (genv L2) s2 t' s2' -> L2 (genv L2) s2 t'' s2'' ->
   (t' = E0 /\ t'' = E0 /\ s2' = s2'')
-  \/ (t' <> E0 /\ t'' <> E0 /\ match_traces ge1 t' t'').
+  \/ (t' <> E0 /\ t'' <> E0 /\ match_traces (genv L1) t' t'').
 Proof.
   intros. 
-  assert (match_traces ge2 t' t'').
+  assert (match_traces (genv L2) t' t'').
     eapply (sd_match determinate); eauto. 
   destruct (silent_or_not_silent t').
   subst. inv H1.  
@@ -1331,15 +1316,15 @@ Proof.
   destruct (silent_or_not_silent t'').
   subst. inv H1. elim H2; auto. 
   right; intuition. 
-  eapply match_traces_preserved with (ge1 := ge2); auto. apply (fsim_symbols_preserved FS). 
+  eapply match_traces_preserved with (ge1 := (genv L2)); auto. apply (fsim_symbols_preserved FS). 
 Qed.
 
 Lemma f2b_determinacy_star:
-  forall s s1, star L2 ge2 s E0 s1 -> 
+  forall s s1, star L2 (genv L2) s E0 s1 -> 
   forall t s2 s3,
-  L2 ge2 s1 t s2 -> t <> E0 ->
-  star L2 ge2 s t s3 ->
-  star L2 ge2 s1 t s3.
+  L2 (genv L2) s1 t s2 -> t <> E0 ->
+  star L2 (genv L2) s t s3 ->
+  star L2 (genv L2) s1 t s3.
 Proof.
   intros s0 s01 ST0. pattern s0, s01. eapply star_E0_ind; eauto.
   intros. inv H3. congruence.
@@ -1352,10 +1337,10 @@ Qed.
 (** Backward simulation of L2 steps *)
 
 Lemma f2b_simulation_step:
-  forall s2 t s2', L2 ge2 s2 t s2' ->
-  forall i s1, f2b_match_states i s1 s2 -> safe L1 ge1 s1 ->
+  forall s2 t s2', L2 (genv L2) s2 t s2' ->
+  forall i s1, f2b_match_states i s1 s2 -> safe L1 (genv L1) s1 ->
   exists i', exists s1',
-    (plus L1 ge1 s1 t s1' \/ (star L1 ge1 s1 t s1' /\ f2b_order i' i))
+    (plus L1 (genv L1) s1 t s1' \/ (star L1 (genv L1) s1 t s1' /\ f2b_order i' i))
      /\ f2b_match_states i' s1' s2'.
 Proof.
   intros s2 t s2' STEP2 i s1 MATCH SAFE.
@@ -1440,7 +1425,7 @@ Qed.
 
 (** The backward simulation *)
 
-Lemma forward_to_backward_simulation: backward_simulation L1 L2 ge1 ge2.
+Lemma forward_to_backward_simulation: backward_simulation L1 L2.
 Proof.
   apply mk_backward_simulation with (bsim_order := f2b_order) (bsim_match_states := f2b_match_states).
   apply wf_f2b_order.
@@ -1469,7 +1454,7 @@ Proof.
 (* simulation *)
   exact f2b_simulation_step.
 (* trace length *)
-  exact (sd_traces determinate ge2).
+  exact (sd_traces determinate).
 (* symbols preserved *)
   exact (fsim_symbols_preserved FS).
 Qed.
